Simplify proof.

Common/Blame.v
@@ -1,6 +1,7 @@
 Require Import Common.Definitions.
 Require Import CompCert.Events.
 Require Import CompCert.Behaviors.
+From mathcomp Require Import ssreflect seq.
 
 Definition extract_finite_trace (beh: program_behavior) : option trace :=
   match beh with
@@ -10,52 +11,14 @@ Definition extract_finite_trace (beh: program_behavior) : option trace :=
   | Goes_wrong t => Some t
   end.
 
-Fixpoint last_event (t: trace) : option event :=
-  match t with
-  | [] => None
-  | [e] => Some e
-  | _::t' => last_event t'
-  end.
-
 Definition who_is_in_control_after (e: event) : Component.id :=
   match e with
   | ECall _ _ _ C => C
   | ERet _ _ C => C
   end.
 
-Definition undef_in
-           (t: trace) (iface: Program.interface) : Prop :=
-  match last_event t with
-  | None =>
-    (* the trace is empty
-       the main component is the only one that we can blame *)
-    Component.main \in (domm iface)
-  | Some e =>
-    (* the last event gives us the component to blame *)
-    (who_is_in_control_after e) \in (domm iface)
-  end.
+Definition last_comp (t: trace) :=
+  last Component.main [seq who_is_in_control_after e | e <- t].
 
-Lemma no_last_event_implies_empty_trace:
-  forall t,
-    last_event t = None -> t = [].
-Proof.
-  intros t Hlast_event.
-  induction t as [|? t' IH].
-  - reflexivity.
-  - destruct t'; simpl in *.
-    + discriminate.
-    + specialize (IH Hlast_event).
-      discriminate.
-Qed.
-
-Lemma last_event_is_in_trace:
-  forall t e,
-    last_event t = Some e -> In e t.
-Proof.
-  intros t e H.
-  induction t.
-  - discriminate.
-  - destruct t; simpl in H.
-    + inversion H. subst. intuition.
-    + apply in_cons. apply IHt. auto.
-Qed.
+Definition undef_in (t: trace) (iface: Program.interface) :=
+  last_comp t \in domm iface.
